src/Prototype/Transaction.v
@@ -10,14 +10,14 @@ Section System.
   Definition postOf (postcond: StateT -> StateT -> Prop): CondT :=
     fun post => forall pre, postcond pre post.
 
-  Definition Separated (c1 c2: CondT) := forall st, c1 st -> c2 st -> False.
-  Infix "-*-" := Separated (at level 30).
+  Definition Disjoint (c1 c2: CondT) := forall st, c1 st -> c2 st -> False.
+  Infix "-*-" := Disjoint (at level 30).
 
   Section PerObject.
     Variable obj: Object MsgT StateT.
 
     Definition Transaction (rq rsr: PMsg MsgT StateT) (rs: MsgId MsgT) :=
-      pmsgOf obj rq /\ pmsgOf obj rsr /\
+      obj_pmsgs obj rq /\ obj_pmsgs obj rsr /\
       (exists st, In rs (outsOf rsr st)) /\
       isTrsPair (midOf rq) rs = true.
 
@@ -31,13 +31,16 @@ Section System.
     | TrsInv: forall rq rsr trsinv,
         postOf (postcondOf rq) --> trsinv ->
         trsinv --> precondOf rsr ->
-        (forall pmsg, pmsgOf obj pmsg -> (precondOf pmsg) -*- trsinv) ->
+        (forall pmsg, obj_pmsgs obj pmsg ->
+                      pmsg <> rsr ->
+                      (precondOf pmsg) -*- trsinv) ->
         TransactionInv rq trsinv rsr.
 
     Definition LocallyDisjoint :=
       forall rq rsr rs,
         Transaction rq rsr rs ->
-        exists trsinv, TransactionInv rq trsinv rsr.
+        exists trsinv,
+          TransactionInv rq trsinv rsr.
 
     Definition MonotonePMsg (pmsg: PMsg MsgT StateT) :=
       match pmsg with
@@ -47,26 +50,52 @@ Section System.
       end.
 
     Definition Monotone :=
-      forall pmsg, pmsgOf obj pmsg -> MonotonePMsg pmsg.
+      forall pmsg, obj_pmsgs obj pmsg -> MonotonePMsg pmsg.
 
   End PerObject.
 
-  Theorem locally_disjoint_linear:
-    forall obj, LocallyDisjoint obj -> Linear (obj :: nil).
+  Section PerSystem.
+    Variable obs: Objects MsgT StateT.
+
+    Theorem sequential_linear: SequentialObs obs -> Linear obs.
+    Proof.
+    Admitted.
+    
+  End PerSystem.
+
+  Theorem locally_disjoint_sequential:
+    forall obj, LocallyDisjoint obj -> SequentialObs (obj :: nil).
   Proof.
   Admitted.
+
+  Corollary locally_disjoint_linear:
+    forall obj, LocallyDisjoint obj -> Linear (obj :: nil).
+  Proof.
+    intros; apply sequential_linear, locally_disjoint_sequential; auto.
+  Qed.
 
 End System.
 
 Section Compositional.
 
-  Theorem linear_compositional:
+  Theorem linear_sequential_compositional:
     forall {MsgT StateT} (obs: Objects MsgT StateT),
-      Forall (fun obj => Monotone obj) obs ->
-      Forall (fun obj => Linear (obj :: nil)) obs ->
+      Forall Monotone obs ->
+      Forall (fun obj => SequentialObs (obj :: nil)) obs ->
       Linear obs.
   Proof.
   Admitted.
+
+  Corollary disjoint_linear:
+    forall {MsgT StateT} (obs: Objects MsgT StateT),
+      Forall Monotone obs ->
+      Forall LocallyDisjoint obs ->
+      Linear obs.
+  Proof.
+    intros; apply linear_sequential_compositional; auto.
+    apply Forall_impl with (P:= LocallyDisjoint); auto.
+    intros; apply locally_disjoint_sequential; auto.
+  Qed.
 
 End Compositional.
 
