src/Prototype/Linearity.v
@@ -1,0 +1,34 @@
+Require Import Bool List String Peano_dec.
+Require Import FnMap Language.
+
+Section History.
+  Variables MsgT StateT: Type.
+
+  Definition Nonlinearizable (hst: list (MsgId MsgT)) :=
+    forall ehst,
+      ExtHistory hst ehst ->
+      forall lhst,
+        Equivalent (complete ehst) lhst ->
+        Concurrent lhst.
+
+  Lemma nonlinearizable_not_linearizable:
+    forall hst, Nonlinearizable hst ->
+                forall lhst, ~ Linearizable hst lhst.
+  Proof.
+    unfold Nonlinearizable, Linearizable; intros.
+    intro Hx; destruct Hx as [ehst [? [? ?]]].
+    specialize (H _ H0 _ H2).
+    auto.
+  Qed.
+
+  Lemma nonlinearizable_ext:
+    forall hst,
+      Nonlinearizable hst ->
+      forall ehst, ExtHistory hst ehst -> Nonlinearizable ehst.
+  Proof.
+    unfold Nonlinearizable; intros.
+    eauto.
+  Qed.
+
+End History.
+
